
# Testing $\sigma^{2}$


## Testing for $\sigma^{2}$

* Parameter of interest: $\sigma^{2}$
* $H_{0}: \sigma^{2} = \sigma_{0}^{2}$
* Assume $Y_{1}, ..., Y_{n}$ are from $\mathcal{N}(\mu, \sigma^{2})$
* Alternative Hypothesis
```math
\begin{align*}
&H_{\alpha}: \sigma^{2} > \sigma_{0}^{2} \Leftrightarrow RR: \{ TS >  \chi^{2}_{\alpha} (n-1) \}  \\
&H_{\alpha}: \sigma^{2} < \sigma_{0}^{2} \Leftrightarrow RR: \{ TS < \chi^{2}_{1- \alpha} (n-1) \}  \\
&H_{\alpha}: \sigma^{2} \neq \sigma_{0}^{2} \Leftrightarrow RR: \{ |TS| > \chi^{2}_{1- \alpha/2} (n-1)\ || \ \chi^{2}_{\alpha/2} (n-1) \}  \\

\end{align*}
```

```math
TS=\frac{(n-1)S^{2}}{\sigma^{2}_{0}}\sim\chi^{2}(n-1)\text{ when }H_{0}\text{ is true }
```

### Case 1: $\sigma^{2} > \sigma_{0}^{2}$

$$\alpha = P \bigg( TS > ts \text{ when } \sigma^{2} = \sigma^{2}_{0} \bigg)$$

$$ts = \chi^{2}_{\alpha} (n-1)$$

### Case 2: $\sigma^{2} < \sigma_{0}^{2}$

$$\alpha = P \bigg( TS < ts \text{ when } \sigma^{2} = \sigma^{2}_{0} \bigg)$$

$$ts = \chi^{2}_{1- \alpha} (n-1)$$

### Case 3: $\sigma^{2} \neq \sigma_{0}^{2}$

```math
\alpha = 
\underbrace{P\bigg(TS<ts_{1}\text{ when }\sigma^{2}=\sigma^{2}_{0}\bigg)}_{\text{ Left tail}} +\underbrace{P\bigg(TS>ts_{2}\text{ when }\sigma^{2}=\sigma^{2}_{0}\bigg)}_{\text{ Right tail}}
```
```math
ts_{1}=\chi^{2}_{1-\alpha/2}(n-1)\quad ts_{2}=\chi^{2}_{\alpha/2}(n-1)
```

## Testing $p$-values for $\sigma^{2}$

* $H_{0}: \sigma^{2} = \sigma^{2}_{0}$
* Alternative Hypothesis
```math
\begin{align*}
&H_{\alpha}: \sigma^{2} > \sigma^{2}_{0} \Leftrightarrow p\text{-value} = P(\chi^{2} > ts) \\
&H_{\alpha}: \sigma^{2} < \sigma^{2}_{0} \Leftrightarrow p\text{-value} = 1- P(\chi^{2} > ts) \\
&H_{\alpha}: \sigma^{2} \neq \sigma^{2}_{0} \Leftrightarrow p\text{-value} = 2\min \bigg[P(\chi^{2} > ts),1- P(\chi^{2} > ts) \bigg]\\
\end{align*}
```

$$TS =\frac{(n-1)S^{2}}{\sigma^{2}_{0}} \sim \chi^{2}(n-1)$$